lib/Lib.Seq.fsti
@@ -13,22 +13,33 @@ let unsnoc (#a: Type) (s: Seq.seq a{
 }) =
   Seq.slice s 0 (Seq.length s - 1)
 
-module List = FStar.List.Tot
+let upd_count (#a: eqtype) (s1 s2: Seq.seq a) (n: nat{n < Seq.length s1}) (x: a): Lemma
+  (requires s2 == Seq.upd s1 n x)
+  (ensures 
+    (x <> Seq.index s1 n ==>
+      Seq.count x s1 + 1 == Seq.count x s2 /\
+      Seq.count (Seq.index s1 n) s1 == Seq.count (Seq.index s1 n) s2 + 1) /\
+    (x == Seq.index s1 n ==> Seq.count x s1 == Seq.count x s2) /\
+    (forall (y: a). {:pattern (Seq.count y s1) \/ (Seq.count y s2)}
+      (y <> x /\ y <> Seq.index s1 n) ==> Seq.count y s1 == Seq.count y s2))
+  [SMTPat (s2 == Seq.upd s1 n x)] =
+  Seq.lemma_count_slice s1 n;
+  Seq.lemma_count_slice s2 n
 
-let no_dup (#a: Type{hasEq a}) (s: Seq.seq a) =
+let no_dup (#a: eqtype) (s: Seq.seq a) =
   forall (x: a). {:pattern Seq.count x s} Seq.mem x s ==> Seq.count x s == 1
 
-let disjoint (#a: Type{hasEq a}) (s1 s2: Seq.seq a) =
-  forall (x: a). {:pattern (Seq.mem x s1); (Seq.mem x s2)}
+let disjoint (#a: eqtype) (s1 s2: Seq.seq a) =
+  forall (x: a). {:pattern (Seq.mem x s1) \/ (Seq.mem x s2)}
     (Seq.mem x s1 ==> Seq.mem x s2 = false) /\
     (Seq.mem x s2 ==> Seq.mem x s1 = false)
 
-let disjoint_comm (#a: Type{hasEq a}) (s1 s2: Seq.seq a): Lemma
+let disjoint_comm (#a: eqtype) (s1 s2: Seq.seq a): Lemma
   (requires disjoint s1 s2)
   (ensures disjoint s2 s1)
   [SMTPat (disjoint s1 s2)] = ()
 
-let no_dup_append (#a: Type{hasEq a}) (s1 s2: Seq.seq a): Lemma
+let no_dup_append (#a: eqtype) (s1 s2: Seq.seq a): Lemma
   (requires no_dup s1 /\ no_dup s2 /\ disjoint s1 s2)
   (ensures no_dup (Seq.append s1 s2))
   [SMTPat (no_dup s1); SMTPat (no_dup s2); SMTPat (disjoint s1 s2)] =
@@ -38,7 +49,7 @@ let no_dup_append (#a: Type{hasEq a}) (s1 s2: Seq.seq a): Lemma
     Seq.append_empty_l s2
   | _ -> Seq.lemma_append_count s1 s2
 
-let no_dup_append' (#a: Type{hasEq a}) (s1 s2: Seq.seq a): Lemma
+let no_dup_append' (#a: eqtype) (s1 s2: Seq.seq a): Lemma
   (requires no_dup (Seq.append s1 s2))
   (ensures no_dup s1 /\ no_dup s2 /\ disjoint s1 s2)
   [SMTPat (no_dup (Seq.append s1 s2))] =
