code/Yazi.Tree.fst
@@ -1,0 +1,125 @@
+module Yazi.Tree
+
+module B = LowStar.Buffer
+module HS = FStar.HyperStack
+module Seq = FStar.Seq
+module SH = Spec.Heap
+module ST = FStar.HyperStack.ST
+module U16 = FStar.UInt16
+module U32 = FStar.UInt32
+module U8 = FStar.UInt8
+
+open FStar.Mul
+open Lib.Seq
+open LowStar.BufferOps
+open Yazi.Tree.Types
+
+let htd_seperate
+  (h: HS.mem) (heap: tree_heap_t)
+  (tree: B.buffer ct_data) (depth: tree_depth_t) =
+  B.live h heap /\ B.live h tree /\ B.live h depth /\
+  B.disjoint heap tree /\ B.disjoint heap depth /\ B.disjoint tree depth
+
+inline_for_extraction
+let smaller
+  (tl: tree_len_t) (tree: B.lbuffer ct_data (Ghost.reveal tl))
+  (depth: tree_depth_t) (n m: U32.t):
+  ST.Stack bool
+  (requires fun h ->
+    U32.v n < tl /\ U32.v m < tl /\
+    B.live h tree /\ B.live h depth)
+  (ensures fun h0 res h1 ->
+    B.modifies B.loc_none h0 h1 /\
+    (res <==> SH.smaller h1 tl tree depth n m)) =
+  let nfd = (tree.(n)).freq_or_dad in
+  let mfd = (tree.(m)).freq_or_dad in
+  if nfd `U16.lt` mfd then
+    true
+  else if nfd `U16.eq` mfd then
+    let dn = depth.(n) in
+    let dm = depth.(m) in
+    dn `U8.lte` dm
+  else
+    false
+
+#set-options "--z3refresh --z3rlimit 32768 --fuel 0 --ifuel 0"
+inline_for_extraction
+let smallest
+  (heap: tree_heap_t) (hl: heap_len_t)
+  (tl: tree_len_t) (tree: B.lbuffer ct_data tl)
+  (depth: tree_depth_t) (i: U32.t{U32.v i < tl})
+  (root: Ghost.erased (heap_internal_index_t hl))
+  (j: heap_internal_index_t hl):
+  ST.Stack U32.t
+  (requires fun h ->
+    let open U32 in
+    v root <= v j /\
+    htd_seperate h heap tree depth /\
+    SH.element_in_range h heap hl tl /\
+    SH.smaller h tl tree depth (B.as_seq h heap).[v j] i /\
+    SH.partial_well_formed h heap hl tl tree depth root)
+  (ensures fun h0 res h1 ->
+    let heap = B.as_seq h1 heap in let hl = U32.v hl in
+    let j = U32.v j in let res = U32.v res in
+    let smaller' = SH.smaller h1 tl tree depth in
+    
+    B.modifies B.loc_none h0 h1 /\
+    res <= hl /\ (res == 0 \/ res == j * 2 \/ res == j * 2 + 1) /\
+    (let k = if res = 0 then i else heap.[res] in
+    k `smaller'` i /\
+    k `smaller'` heap.[j * 2] /\
+    (j * 2 + 1 <= hl ==> k `smaller'` heap.[j * 2 + 1]) /\
+    heap.[j] `smaller'` k)) =
+  let open U32 in
+  let l = j *^ 2ul in
+  let r = l +^ 1ul in
+  let le = heap.(l) in
+  let smaller' = smaller tl tree depth in
+  if r >^ hl then
+    if i `smaller'` le then 0ul else l
+  else
+    let re = heap.(r) in
+    if i `smaller'` le then
+      if i `smaller'` re then 0ul else r
+    else
+      if le `smaller'` re then l else r
+
+#set-options "--z3refresh --z3rlimit 32768 --fuel 0 --ifuel 0"
+[@CInline]
+let rec do_pqdownheap
+  (h_init: Ghost.erased HS.mem)
+  (heap: tree_heap_t) (hl: heap_len_t)
+  (tl: tree_len_t) (tree: B.lbuffer ct_data tl)
+  (depth: tree_depth_t)
+  (i: U32.t{U32.v i < tl})
+  (k: Ghost.erased (heap_internal_index_t hl))
+  (j: heap_index_t hl):
+  ST.Stack unit
+  (requires fun h ->
+    let open U32 in
+    v k <= v j /\
+    (B.as_seq h_init heap).[v k] == i /\
+    htd_seperate h heap tree depth /\
+    SH.smaller h tl tree depth (B.as_seq h heap).[U32.v j] i /\
+    SH.partial_well_formed h heap hl tl tree depth k /\
+    SH.permutation_partial (B.as_seq h_init heap) (B.as_seq h heap) k j)
+  (ensures fun h0 _ h1 ->
+    B.modifies (B.loc_buffer heap) h0 h1 /\
+    SH.partial_well_formed h1 heap hl tl tree depth k)
+  (decreases U32.v hl / 2 - U32.v j) =
+  let open U32 in
+  let internal = hl /^ 2ul in
+  if j >^ internal then
+    heap.(j) <- i
+  else
+    let s = smallest heap hl tl tree depth i k j in
+    if s = 0ul then
+      heap.(j) <- i
+    else begin
+      let h0 = ST.get () in
+      let s' = heap.(s) in
+      heap.(j) <- s';
+      let h1 = ST.get () in
+      upd_count (B.as_seq h0 heap) (B.as_seq h1 heap) (v j) s';
+      do_pqdownheap h_init heap hl tl tree depth i k s
+    end
