specs/Spec.Heap.fst
@@ -1,0 +1,57 @@
+module Spec.Heap
+
+module B = LowStar.Buffer
+module HS = FStar.HyperStack
+module U16 = FStar.UInt16
+module U32 = FStar.UInt32
+module U8 = FStar.UInt8
+
+open FStar.Mul
+open FStar.Seq
+open Lib.Seq
+open Yazi.Tree.Types
+
+let smaller (h: HS.mem)
+  (tl: nat) (tree: B.lbuffer ct_data tl)
+  (depth: tree_depth_t) (i j: U32.t) =
+  let open U32 in
+  let tree = B.as_seq h tree in
+  let depth = B.as_seq h depth in
+  v i < tl /\ v j < tl /\ v i < length depth /\ v j < length depth /\
+  (let fi = U16.v (tree.[v i]).freq_or_dad in
+  let fj = U16.v (tree.[v j]).freq_or_dad in
+  (fi < fj \/ (fi == fj /\ U8.v depth.[v i] <= U8.v depth.[v j])))
+
+let element_in_range (h: HS.mem) (heap: tree_heap_t) (hl: heap_len_t) (tl: nat) =
+  let heap = B.as_seq h heap in
+  (forall (j: pos). {:pattern heap.[j]} j <= U32.v hl ==> U32.v heap.[j] < tl)
+
+let partial_well_formed
+  (h: HS.mem)
+  (heap: tree_heap_t) (hl: heap_len_t)
+  (tl: nat) (tree: B.lbuffer ct_data tl) (depth: tree_depth_t)
+  (i: heap_index_t hl) =
+  let open U32 in
+  let heap' = B.as_seq h heap in
+  element_in_range h heap hl tl /\
+  (forall (k: nat). (v i <= k /\ k <= v hl) ==> (
+    (k * 2 <= v hl ==> smaller h tl tree depth heap'.[k] heap'.[k * 2]) /\
+    (k * 2 + 1 <= v hl ==> smaller h tl tree depth heap'.[k] heap'.[k * 2 + 1])))
+
+let well_formed
+  (h: HS.mem) (heap: tree_heap_t) (hl: heap_len_t)
+  (tl: nat) (tree: B.lbuffer ct_data tl) (depth: tree_depth_t) =
+  U32.v hl > 1 ==> partial_well_formed h heap hl tl tree depth 1ul
+
+unfold let permutation_partial (h1 h2: seq U32.t) (root hole: U32.t) =
+  let root = U32.v root in let hole = U32.v hole in
+  length h1 == length h2 /\
+  root <= hole /\ hole < length h1 /\
+  (hole == root ==> Seq.permutation U32.t h1 h2 /\ h1 == h2) /\
+  (hole <> root ==> 
+    (h2.[hole] <> h1.[root] ==>
+      count h1.[root] h2 + 1 == count h1.[root] h1 /\
+      count h2.[hole] h2 == count h2.[hole] h1 + 1) /\
+    (h2.[hole] == h1.[root] ==> count h1.[root] h2 == count h1.[root] h1) /\
+    (forall (x: U32.t). {:pattern (count x h1) \/ (count x h2)}
+      (x <> h1.[root] /\ x <> h2.[hole]) ==> count x h1 == count x h2))
